Transformations/Alpha_Equiv_Bigstep_Correct.thy
@@ -37,32 +37,11 @@ fun alpha_equiv_local_variables'l ::
       (val1 = val2 \<and> alpha_equiv_local_variables'l nt vm1 vm2)))"
 *)
 
-definition alpha_equiv_local_variables' ::
-  "(name, name) oalist \<Rightarrow> (Identifier * Value) list \<Rightarrow> (Identifier * Value) list \<Rightarrow> bool" where
-"alpha_equiv_local_variables' subst vm1 vm2 =
-  (oalist_all (\<lambda> (n1, n2) .
-    (case map_of vm1 n1 of
-      None \<Rightarrow> False
-      | Some val1 \<Rightarrow>
-        (case map_of vm2 n2 of
-          None \<Rightarrow> False
-          | Some val2 \<Rightarrow> val1 = val2))) subst)"
-
-(* make sure that our oalist substitution captures all the local variables. *)
-
 definition alpha_equiv_local_variables ::
-  "subst \<Rightarrow> (Identifier * Value) list \<Rightarrow> (Identifier * Value) list \<Rightarrow> bool" where
+  "(name * name) list \<Rightarrow> (Identifier * Value) list \<Rightarrow> (Identifier * Value) list \<Rightarrow> bool" where
 "alpha_equiv_local_variables subst vm1 vm2 =
-  (list_all (\<lambda> subst' . alpha_equiv_local_variables' subst' vm1 vm2) subst \<and>
-   list_all oalist_one_one subst \<and>
-   list_all (\<lambda> (k, v) . 
-    (case subst_get subst k of
-      Some _ \<Rightarrow> True
-      | _ \<Rightarrow> False)) vm1 \<and>
-   list_all (\<lambda> (k, v) . 
-    (case subst_get (map oalist_flip subst) k of
-      Some _ \<Rightarrow> True
-      | _ \<Rightarrow> False)) vm2)"
+  (subst = zip (map fst vm1) (map fst vm2) \<and>
+   map snd vm1 = map snd vm2)"
 
 (* function equivalence
 *)
@@ -70,45 +49,110 @@ definition alpha_equiv_local_variables ::
 type_synonym FunctionContext =
   \<open>(Identifier\<times> (Statement \<times> Identifier list)) list\<close>
 
+type_synonym 'g BuiltinContext =
+  \<open>Identifier \<Rightarrow> ('g BuiltinFunction) option\<close>
+
 (* TODO: make sure that the way we are making use of the "visible"
  * identifiers is correct.
  *)
-definition alpha_equiv_function_contexts' ::
-  "(name, name) oalist \<Rightarrow> FunctionContext \<Rightarrow> FunctionContext \<Rightarrow> bool" where
-"alpha_equiv_function_contexts' subst vm1 vm2 =
-  oalist_all (\<lambda> (n1, n2) .
-    (case map_of vm1 n1 of
-      None \<Rightarrow> False
-      | Some (FunctionDefinition n1' params1 rets1 body1, ids1) \<Rightarrow>
-        (case map_of vm2 n2 of
-          None \<Rightarrow> False
-          | Some (FunctionDefinition n2' params2 rets2 body2, ids2) \<Rightarrow> 
-            (n1 = n1' \<and> n2 = n2' \<and>
-            alpha_equiv_statement [to_oalist (zip ids1 ids2)] [Oalist.empty]
-              (FunctionDefinition n1' params1 rets1 body1)
-              (FunctionDefinition n2' params2 rets2 body2))))) subst"
-
 definition alpha_equiv_function_contexts ::
-  "subst \<Rightarrow> FunctionContext \<Rightarrow> FunctionContext \<Rightarrow> bool" where
+  "(name * name) list \<Rightarrow> FunctionContext \<Rightarrow> FunctionContext \<Rightarrow> bool" where
 "alpha_equiv_function_contexts subst vm1 vm2 =
-  (list_all (\<lambda> subst' . alpha_equiv_function_contexts' subst' vm1 vm2) subst \<and>
-   list_all (\<lambda> (k, v) . 
-    (case subst_get subst k of
-      Some _ \<Rightarrow> True
-      | _ \<Rightarrow> False)) vm1 \<and>
-   list_all (\<lambda> (k, v) . 
-    (case subst_get (map oalist_flip subst) k of
-      Some _ \<Rightarrow> True
-      | _ \<Rightarrow> False)) vm2)"
+  (subst = zip (map fst vm1) (map fst vm2) \<and>
+   list_all2
+    (\<lambda> (n1, f1) (n2, f2) .
+      (case f1 of
+        (FunctionDefinition n1' params1 rets1 body1, ids1) \<Rightarrow>
+        (case f2 of
+          (FunctionDefinition n2' params2 rets2 body2, ids2) \<Rightarrow>
+            (n1 = n1' \<and> n2 = n2' \<and>
+            alpha_equiv_statement (zip ids1 ids2) []
+              (FunctionDefinition n1' params1 rets1 body1)
+              (FunctionDefinition n2' params2 rets2 body2))        
+        | _ \<Rightarrow> False)
+      | _ \<Rightarrow> False)) vm1 vm2)"
 
-(* TODO: ignoring builtins for now *)
+definition alpha_equiv_builtin_contexts ::
+   "(name * name) list \<Rightarrow> 'g BuiltinContext \<Rightarrow> 'g BuiltinContext \<Rightarrow> bool" where
+"alpha_equiv_builtin_contexts subst vm1 vm2 =
+  ((\<forall> n f . vm1 n = Some f \<longrightarrow> n \<in> set (map fst subst)) \<and>
+   (\<forall> n f . vm2 n = Some f \<longrightarrow> n \<in> set (map snd subst)) \<and>
+   list_all (\<lambda> (n1, n2) . vm1 n1 = vm2 n2) subst)"
+
+lemma alpha_equiv_builtin_contextsI :
+  fixes vm1 vm2 :: "'g BuiltinContext"
+  assumes "\<And> n f . vm1 n = Some f \<Longrightarrow> n \<in> set (map fst subst)" 
+  assumes "\<And> n f . vm2 n = Some f \<Longrightarrow> n \<in> set (map snd subst)"
+  assumes "list_all (\<lambda> (n1, n2) . vm1 n1 = vm2 n2) subst"
+  shows "alpha_equiv_builtin_contexts subst vm1 vm2"
+  using assms
+  unfolding alpha_equiv_builtin_contexts_def
+  by blast
+
+lemma alpha_equiv_builtin_contextsD :
+  fixes vm1 vm2 :: "'g BuiltinContext"
+  assumes "alpha_equiv_builtin_contexts subst vm1 vm2"
+  shows
+  "\<And> n f . vm1 n = Some f \<Longrightarrow> n \<in> set (map fst subst)" 
+  "\<And> n f . vm2 n = Some f \<Longrightarrow> n \<in> set (map snd subst)"
+  "list_all (\<lambda> (n1, n2) . vm1 n1 = vm2 n2) subst"
+  using assms
+  unfolding alpha_equiv_builtin_contexts_def
+  by(auto)
+
 definition alpha_equiv_yulcontext ::
   "subst \<Rightarrow> subst \<Rightarrow> 'g yulcontext \<Rightarrow> 'g yulcontext \<Rightarrow> bool" where
 "alpha_equiv_yulcontext fsubst vsubst c1 c2 =
  (GlobalState c1 = GlobalState c2 \<and>
   alpha_equiv_Result (Status c1) (Status c2) \<and>
   alpha_equiv_local_variables vsubst (LocalVariables c1) (LocalVariables c2)\<and>
-  alpha_equiv_function_contexts fsubst (Functions c1) (Functions c2))"
+  alpha_equiv_function_contexts fsubst (Functions c1) (Functions c2) \<and>
+  alpha_equiv_builtin_contexts fsubst (BuiltinFunctions c1) (BuiltinFunctions c2))"
+
+lemma alpha_equiv_yulcontextI :
+  assumes "GlobalState c1 = GlobalState c2"
+  assumes "alpha_equiv_Result (Status c1) (Status c2)"
+  assumes "alpha_equiv_local_variables vsubst (LocalVariables c1) (LocalVariables c2)"
+  assumes "alpha_equiv_function_contexts fsubst (Functions c1) (Functions c2)"
+  assumes "alpha_equiv_builtin_contexts fsubst (BuiltinFunctions c1) (BuiltinFunctions c2)"
+  shows "alpha_equiv_yulcontext fsubst vsubst c1 c2"
+  using assms
+  unfolding alpha_equiv_yulcontext_def
+  by auto
+
+lemma alpha_equiv_yulcontextD :
+  assumes "alpha_equiv_yulcontext fsubst vsubst c1 c2"
+  shows 
+    "GlobalState c1 = GlobalState c2"
+    "alpha_equiv_Result (Status c1) (Status c2)"
+    "alpha_equiv_local_variables vsubst (LocalVariables c1) (LocalVariables c2)"
+    "alpha_equiv_function_contexts fsubst (Functions c1) (Functions c2)"
+    "alpha_equiv_builtin_contexts fsubst (BuiltinFunctions c1) (BuiltinFunctions c2)"
+  using assms
+  unfolding alpha_equiv_yulcontext_def
+  by auto
+
+lemma find_map_of :
+  "map_option snd (find (\<lambda> (declaredName,_) . declaredName = idn) l) =
+   map_of l idn"
+proof(induction l arbitrary: idn)
+  case Nil
+  then show ?case
+    by(auto)
+next
+  case (Cons lh lt)
+
+  obtain lhk lhv where Lh : "lh = (lhk, lhv)"
+    by(cases lh; auto)
+
+  show ?case using Cons Lh
+    by(auto)
+qed
+
+lemma getLocalVariable_alt_def :
+  shows "getLocalVariable c n = map_of (LocalVariables c) n"
+  unfolding getLocalVariable_def
+  by(auto simp add: find_map_of)
 
 (* result of running the state monad *)
 type_synonym ('g, 'a) yulout = "('a * 'g yulcontext)"
@@ -116,54 +160,111 @@ type_synonym ('g, 'a) yulout = "('a * 'g yulcontext)"
 (* for unpacking the State constructor *)
 type_synonym ('g, 'a) yulstatef = "'g yulcontext \<Rightarrow> ('a * 'g yulcontext)"
 
-lemma alpha_equiv_getLocalVariable :
+lemma alpha_equiv_getLocalVariable' :
   assumes "alpha_equiv_local_variables vsubst lv1 lv2"
   assumes "LocalVariables c1 = lv1"
   assumes "LocalVariables c2 = lv2"
   assumes "alpha_equiv_name vsubst id1 id2"
   shows "getLocalVariable c1 id1 = getLocalVariable c2 id2"
   using assms
-  sorry
-(*
-proof(induction lv1 arbitrary: vsubst lv2 c1 c2 id1 id2)
+proof(induction vsubst arbitrary: lv1 lv2 c1 c2 id1 id2)
   case Nil1 : Nil
   then show ?case
-    apply(auto simp add: alpha_equiv_local_variables_def)
+    by(auto simp add: alpha_equiv_local_variables_def getLocalVariable_def)
 next
   case (Cons substh substt)
+
+  obtain substhn1 substhn2 where Substh : "substh = (substhn1, substhn2)"
+    by(cases substh; auto)
+
+  obtain lv1h lv1t where Lv1 : "lv1 = lv1h # lv1t"
+    using Cons.prems
+    by(cases lv1; auto simp add: alpha_equiv_local_variables_def)
+
+  obtain lv1hk lv1hv where Lv1h : "lv1h = (lv1hk, lv1hv)"
+    by(cases lv1h; auto)
+
+  obtain lv2h lv2t where Lv2 : "lv2 = lv2h # lv2t"
+    using Cons.prems
+    by(cases lv2; auto simp add: alpha_equiv_local_variables_def)
+
+  obtain lv2hk lv2hv where Lv2h : "lv2h = (lv2hk, lv2hv)"
+    by(cases lv2h; auto)
+
   show ?case
-  proof(cases "get substh id1")
-    case None1 : None
-
-    show ?thesis
-    proof(cases "get (oalist_flip substh) id2")
-      case None2 : None
-      then show ?thesis
-        using Cons None1
-        apply(auto simp add: alpha_equiv_local_variables_def)
-    next
-      case (Some a)
-      then show ?thesis sorry
-    qed
-
+  proof(cases "id1 = lv1hk")
+    case Eq1 : True
     then show ?thesis
-      using Cons
-      apply(auto simp add: alpha_equiv_local_variables_def)
-    then show ?thesis sorry
+      using Cons Substh Lv1 Lv1h Lv2 Lv2h
+      by(auto simp add: alpha_equiv_name_def alpha_equiv_local_variables_def getLocalVariable_alt_def split: option.splits)
   next
-    case Some1 : (Some id1')
+    case Neq1 : False
 
     show ?thesis
-      using Cons
-      apply(auto simp add: alpha_equiv_local_variables_def)
-
-    then show ?thesis sorry
+    proof(cases "id2 = lv2hk")
+      case Eq2 : True
+      then show ?thesis
+        using Cons Substh Lv1 Lv1h Lv2 Lv2h Neq1
+        by(auto simp add: alpha_equiv_name_def alpha_equiv_local_variables_def getLocalVariable_alt_def flip_def split: option.splits)
+    next
+      case Neq2 : False
+      then show ?thesis
+        using Cons.prems Cons.IH[of lv1t lv2t "c1 \<lparr> LocalVariables := lv1t \<rparr>" "c2 \<lparr> LocalVariables := lv2t \<rparr>"] Substh Lv1 Lv1h Lv2 Lv2h Neq1
+        by(auto simp add: alpha_equiv_name_def alpha_equiv_local_variables_def getLocalVariable_alt_def flip_def split: option.splits)
+    qed
   qed
-
-  then show ?case
-    apply(auto simp add: alpha_equiv_local_variables_def)
 qed
-*)
+
+lemma alpha_equiv_getLocalVariable :
+  assumes "alpha_equiv_local_variables vsubst (LocalVariables c1) (LocalVariables c2)"
+  assumes "alpha_equiv_name vsubst id1 id2"
+  shows "getLocalVariable c1 id1 = getLocalVariable c2 id2"
+  using assms alpha_equiv_getLocalVariable'
+  by blast
+
+lemma alpha_equiv_name_In :
+  assumes "alpha_equiv_name subst n1 n2"
+  shows "(n1, n2) \<in> set subst"
+  using assms
+proof(induction subst arbitrary: n1 n2)
+  case Nil
+  then show ?case
+    by(auto simp add: alpha_equiv_name_def)
+next
+  case (Cons substh substt)
+
+  obtain substh1 substh2 where Substh : "substh = (substh1, substh2)"
+    by force
+
+  show ?case
+  proof(cases "substh1 = n1")
+    case Eq1 : True
+
+    show ?thesis
+    proof(cases "n2 = substh2")
+      case Eq2 : True
+      then show ?thesis using Cons Substh Eq1
+        by(auto simp add: alpha_equiv_name_def flip_def)
+    next
+      case Neq2 : False
+      then show ?thesis using Cons Substh Eq1
+        by(cases "map_of (map (\<lambda>(x, y). (y, x)) substt) n2"; auto simp add: alpha_equiv_name_def flip_def)
+    qed
+  next
+    case Neq1 : False
+
+    show ?thesis
+    proof(cases "n2 = substh2")
+      case Eq2 : True
+      then show ?thesis using Cons Substh Neq1
+        by(cases "map_of substt n1"; auto simp add: alpha_equiv_name_def flip_def)
+    next
+      case Neq2 : False
+      then show ?thesis using Cons Substh Neq1
+        by(auto simp add: alpha_equiv_name_def flip_def)
+    qed
+  qed
+qed
 
 (* State_Monad.state.rel_state :: "('a \<Rightarrow> 'b \<Rightarrow> bool) \<Rightarrow> ('c, 'a) state \<Rightarrow> ('c, 'b) state \<Rightarrow> bool" *)
 (* run_state :: "('s, 'a) state \<Rightarrow> 's \<Rightarrow> 'a \<times> 's" *)
@@ -199,19 +300,71 @@ next
 
   have IH1 :
     "\<And> fsubst vsubst (c1 :: 'g yulcontext) (c2 :: 'g yulcontext) st1 st2 m m1 m2 c1' c2'.
-         alpha_equiv_statement fsubst vsubst
-          st1 st2 \<Longrightarrow>
-         alpha_equiv_yulcontext fsubst vsubst
-          c1 c2 \<Longrightarrow>
-         run_state (evalStatement n m st1) c1 =
-         (m1, c1') \<Longrightarrow>
-         run_state (evalStatement n m st2) c2 =
-         (m2, c2') \<Longrightarrow>
-         alpha_equiv_yulcontext fsubst vsubst
-          c1' c2' \<and>
-         m1 = m2"
+       alpha_equiv_statement fsubst vsubst st1 st2 \<Longrightarrow>
+       alpha_equiv_yulcontext fsubst vsubst c1 c2 \<Longrightarrow>
+       run_state (evalStatement n m st1) c1 = (m1, c1') \<Longrightarrow>
+       run_state (evalStatement n m st2) c2 = (m2, c2') \<Longrightarrow>
+       alpha_equiv_yulcontext fsubst vsubst c1' c2' \<and> m1 = m2"
     using Suc.IH
     by fast
+
+  have IH1_traverse_mode :
+    "\<And> fsubst vsubst (c1 :: 'g yulcontext) (c2 :: 'g yulcontext) l1 l2 m m1 m2 c1' c2'.
+       list_all2 (alpha_equiv_statement fsubst vsubst) l1 l2 \<Longrightarrow>
+       alpha_equiv_yulcontext fsubst vsubst c1 c2 \<Longrightarrow>
+       run_state (traverse_list_mode (evalStatement n m) l1) c1 = (m1, c1') \<Longrightarrow>
+       run_state (traverse_list_mode (evalStatement n m) l2) c2 = (m2, c2') \<Longrightarrow>
+       alpha_equiv_yulcontext fsubst vsubst c1' c2' \<and> m1 = m2"
+  proof-
+    fix fsubst vsubst
+    fix c1 c2 :: "'g yulcontext"
+    fix l1 l2 m m1 m2 c1' c2'
+
+    show "list_all2 (alpha_equiv_statement fsubst vsubst) l1 l2 \<Longrightarrow>
+       alpha_equiv_yulcontext fsubst vsubst c1 c2 \<Longrightarrow>
+       run_state (traverse_list_mode (evalStatement n m) l1) c1 = (m1, c1') \<Longrightarrow>
+       run_state (traverse_list_mode (evalStatement n m) l2) c2 = (m2, c2') \<Longrightarrow>
+       alpha_equiv_yulcontext fsubst vsubst c1' c2' \<and> m1 = m2"
+    proof(induction l1 arbitrary: fsubst vsubst c1 c2 l2 m m1 m2 c1' c2')
+      case Nil1 : Nil
+      then show ?case by auto
+    next
+      case Cons1 : (Cons l1h l1t)
+
+      obtain l2h l2t where Cons2 : "l2 = l2h # l2t"
+        using Cons1.prems
+        by(cases l2; auto)
+
+      obtain c1h m1h where Run1 : "run_state (evalStatement n m l1h) c1 = (m1h, c1h)"
+        by force
+
+      obtain c2h m2h where Run2 : "run_state (evalStatement n m l2h) c2 = (m2h, c2h)"
+        by force
+
+      have Result : "alpha_equiv_yulcontext fsubst vsubst c1h c2h" "m1h = m2h"
+        using IH1[OF _ _ Run1 Run2, of fsubst vsubst] Cons1.prems Cons2
+        by(auto)
+
+      obtain c1t m1t where Run1t : "run_state (traverse_list_mode (evalStatement n m1h) l1t) c1h = (m1t, c1t)"
+        by force
+
+      obtain c2t m2t where Run2t : "run_state (traverse_list_mode (evalStatement n m1h) l2t) c2h = (m2t, c2t)"
+        by force
+
+      show ?case
+      proof(cases "m1h = RegularMode")
+        case True
+        then show ?thesis 
+          using Cons1.prems Cons2 Run1 Run2 Cons1.IH[OF _ Result(1) Run1t Run2t] Result Run1t Run2t
+          by(cases m; auto)
+      next
+        case False
+        then show ?thesis
+          using Cons1.prems Cons2 Run1 Run2 Result Run1t Run2t
+          by(cases m; auto)
+      qed
+    qed
+  qed
 
   have IH2 :
     "\<And> fsubst vsubst (c1 :: 'g yulcontext) (c2 :: 'g yulcontext) e1 e2 c1' c2' vals1 vals2.
@@ -223,6 +376,8 @@ next
     using Suc.IH
     by fast
 
+  (* IH2_traverse is probably not needed. *)
+
   have IH3 :
     "\<And> fsubst vsubst (c1 :: 'g yulcontext) (c2 :: 'g yulcontext) e1 e2 c1' c2' v1 v2.
     alpha_equiv_expr fsubst vsubst e1 e2 \<Longrightarrow>
@@ -232,6 +387,57 @@ next
     alpha_equiv_yulcontext fsubst vsubst c1' c2' \<and> v1 = v2"
     using Suc.IH
     by fast
+
+  have IH3_traverse :
+    "\<And> fsubst vsubst (c1 :: 'g yulcontext) (c2 :: 'g yulcontext) l1 l2 c1' c2' v1 v2 .
+    list_all2 (alpha_equiv_expr fsubst vsubst) l1 l2 \<Longrightarrow>
+    alpha_equiv_yulcontext fsubst vsubst c1 c2 \<Longrightarrow>
+    run_state (traverse_list (evalUnaryExpression n) l1) c1 = (v1, c1') \<Longrightarrow>
+    run_state (traverse_list (evalUnaryExpression n) l2) c2 = (v2, c2') \<Longrightarrow>
+    alpha_equiv_yulcontext fsubst vsubst c1' c2' \<and> v1 = v2"
+  proof-
+    fix fsubst vsubst
+    fix c1 c2 :: "'g yulcontext"
+    fix l1 l2 c1' c2' v1 v2
+    show "list_all2 (alpha_equiv_expr fsubst vsubst) l1 l2 \<Longrightarrow>
+       alpha_equiv_yulcontext fsubst vsubst c1 c2 \<Longrightarrow>
+       run_state (traverse_list (evalUnaryExpression n) l1) c1 =
+       (v1, c1') \<Longrightarrow>
+       run_state (traverse_list (evalUnaryExpression n) l2) c2 =
+       (v2, c2') \<Longrightarrow>
+       alpha_equiv_yulcontext fsubst vsubst c1' c2' \<and> v1 = v2"
+    proof(induction l1 arbitrary: fsubst vsubst c1 c2 l2 c1' c2' v1 v2)
+      case Nil1 : Nil
+      then show ?case 
+        by(auto)
+    next
+      case Cons1 : (Cons l1h l1t)
+
+      obtain l2h l2t where Cons2 : "l2 = l2h # l2t"
+        using Cons1.prems
+        by(cases l2; auto)
+
+      obtain c1h v1h where Run1 : "run_state (evalUnaryExpression n l1h) c1 = (v1h, c1h)"
+        by force
+
+      obtain c2h v2h where Run2 : "run_state (evalUnaryExpression n l2h) c2 = (v2h, c2h)"
+        by force
+
+      have Result : "alpha_equiv_yulcontext fsubst vsubst c1h c2h" "v1h = v2h"
+        using IH3[OF _ _ Run1 Run2, of fsubst vsubst] Cons1.prems Cons2
+        by(auto)
+
+      obtain c1t v1t where Run1t : "run_state (traverse_list (evalUnaryExpression n) l1t) c1h = (v1t, c1t)"
+        by force
+
+      obtain c2t v2t where Run2t : "run_state (traverse_list (evalUnaryExpression n) l2t) c2h = (v2t, c2t)"
+        by force
+
+      show ?case 
+        using Cons1.prems Cons2 Run1 Run2 Cons1.IH[OF _ Result(1) Run1t Run2t] Result(2) Run1t Run2t
+        by(auto)
+    qed
+  qed
 
   have Conc1 : 
     "\<And> fsubst vsubst (c1 :: 'g yulcontext) (c2 :: 'g yulcontext)
@@ -279,8 +485,84 @@ next
     show "alpha_equiv_yulcontext fsubst vsubst c1' c2' \<and>
        vals1 = vals2"
     proof(cases e1)
-      case Fc1 : (FunctionCall x11 x12)
-      then show ?thesis sorry
+      case Fc1 : (FunctionCall f1 args1)
+
+      then obtain f2 args2 where Fc2 : "e2 = FunctionCall f2 args2"
+        using Hexpr
+        by(cases e2; auto)
+
+      have Fname : "alpha_equiv_name fsubst f1 f2"
+        using Fc1 Fc2 Hexpr
+        by auto
+
+      hence Fname_In : "(f1, f2) \<in> set fsubst"
+        using alpha_equiv_name_In
+        by auto
+
+      obtain argvals1 argsc1 where Args1 :
+        "run_state (traverse_list (evalUnaryExpression n) (rev args1)) c1 = (argvals1, argsc1)"
+        by force
+
+      obtain argvals2 argsc2 where Args2 :
+        "run_state (traverse_list (evalUnaryExpression n) (rev args2)) c2 = (argvals2, argsc2)"
+        by force
+
+      have Equiv_after_args :
+        "alpha_equiv_yulcontext fsubst vsubst argsc1 argsc2" "argvals1 = argvals2"
+        using IH3_traverse[OF _ _ Args1 Args2, of fsubst vsubst] Hexpr Hctx Fc1 Fc2
+        by(auto)
+
+      obtain bivals1_o biresc1 where Builtin1 : "run_state (BuiltinFunctionOfIdentifier f1) argsc1 = (bivals1_o, biresc1)"
+        by force
+
+      obtain bivals2_o biresc2 where Builtin2 : "run_state (BuiltinFunctionOfIdentifier f2) argsc2 = (bivals2_o, biresc2)"
+        by force
+
+      show ?thesis
+      proof(cases bivals1_o)
+        case Isnt_builtin1 : None
+
+        have Isnt_builtin1' : "BuiltinFunctions argsc1 f1 = None"
+          using Hexpr Hctx Hrun1 Hrun2 Fc1 Fc2 Args1 Args2 Builtin1 Builtin2 Isnt_builtin1
+          by(cases "BuiltinFunctions argsc1 f1"; auto simp add: alpha_equiv_yulcontext_def alpha_equiv_function_contexts_def BuiltinFunctionOfIdentifier_def)
+
+        have Argsc_builtins : "list_all (\<lambda>(n1, n2). BuiltinFunctions argsc1 n1 = BuiltinFunctions argsc2 n2) fsubst"
+          using Equiv_after_args
+          by(auto simp add: alpha_equiv_yulcontext_def alpha_equiv_builtin_contexts_def)
+
+        have Isnt_builtin2' : "BuiltinFunctions argsc2 f2 = None"
+          using Argsc_builtins Fname_In Isnt_builtin1'
+          unfolding list_all_iff
+          by(auto)
+
+        have Isnt_builtin2 : "bivals2_o = None"
+          using Hexpr Hctx Hrun1 Hrun2 Fc1 Fc2 Args1 Args2 Builtin1 Builtin2 Isnt_builtin1 Isnt_builtin1' Isnt_builtin2'
+          by(cases bivals2_o; auto simp add: BuiltinFunctionOfIdentifier_def)
+
+        show ?thesis using Hexpr Hctx Hrun1 Hrun2 Fc1 Fc2 Args1 Args2 Builtin1 Builtin2 Isnt_builtin1' Isnt_builtin2'
+          apply(auto simp add: alpha_equiv_yulcontext_def alpha_equiv_function_contexts_def BuiltinFunctionOfIdentifier_def)
+
+(*
+        then have Isnt_builtin2' : "BuiltinFunctions argsc2 f2 = None"
+          using Equiv_after_args Hexpr Fc1 Fc2
+          apply(auto simp add: alpha_equiv_yulcontext_def alpha_equiv_function_contexts)
+
+        have Isnt_builtin2 : "bivals2_o = None"
+          using Hexpr Hctx Hrun1 Hrun2 Fc1 Fc2 Args1 Args2 Builtin1 Builtin2 Isnt_builtin1 Isnt_builtin1'
+          apply(auto simp add: alpha_equiv_yulcontext_def alpha_equiv_function_contexts_def BuiltinFunctionOfIdentifier_def)
+
+        show ?thesis
+          using Hexpr Hctx Hrun1 Hrun2 Fc1 Fc2 Args1 Args2 Builtin1 Builtin2 Isnt_builtin1
+          apply(auto simp add: errorState_def alpha_equiv_yulcontext_def)
+*)
+      next
+        case Is_builtin1 : (Some bivals1)
+        then show ?thesis sorry
+      qed
+
+        using Hexpr Hctx Hrun1 Hrun2 Fc1 Fc2 Args1 Args2 Builtin1 Builtin2
+        apply(auto simp add: errorState_def alpha_equiv_yulcontext_def)
+
     next
       case Id1 : (Identifier i1)
 
@@ -288,29 +570,39 @@ next
         using Hexpr
         by(cases e2; auto)
 
+      have Locals :
+        "alpha_equiv_local_variables vsubst (LocalVariables c1) (LocalVariables c2)"
+        using Hctx
+        by(auto simp add: alpha_equiv_yulcontext_def)
+
+      have Names :
+        "alpha_equiv_name vsubst i1 i2"
+        using Hexpr Id1 Id2
+        by(auto)
+
       show ?thesis
       proof(cases "getLocalVariable c1 i1")
         case None1 : None
 
-(* need lemma relating getLocalVariable to alpha_equiv_local_variables *)
+        (* need lemma relating getLocalVariable to alpha_equiv_local_variables *)
         then have None2 : "getLocalVariable c2 i2 = None"
-          using Hexpr Hrun1 Hrun2 Id1 Id2 Hctx
-          apply(cases "getLocalVariable c2 i2"; auto simp add: errorState_def alpha_equiv_yulcontext_def ValueOfIdentifier_def)
+          using alpha_equiv_getLocalVariable[OF Locals Names]
+          by auto
+
         then show ?thesis
-          using Hexpr Hrun1 Hrun2 Id1 Id2
-          apply(auto simp add: errorState_def alpha_equiv_yulcontext_def ValueOfIdentifier_def)
-
+          using Hctx Hexpr Hrun1 Hrun2 Id1 Id2 None1
+          by(auto simp add: errorState_def alpha_equiv_yulcontext_def ValueOfIdentifier_def)
       next
-        case (Some a)
-        then show ?thesis sorry
+        case Some1 : (Some v1)
+
+        then have Some2 : "getLocalVariable c2 i2 = Some v1"
+          using alpha_equiv_getLocalVariable[OF Locals Names]
+          by auto
+
+        then show ?thesis
+          using Hctx Hexpr Hrun1 Hrun2 Id1 Id2 Some1
+          by(auto simp add: errorState_def alpha_equiv_yulcontext_def ValueOfIdentifier_def)
       qed
-
-(* get_local_variable *)
-      then show ?thesis using Hexpr Hctx Hrun1 Hrun2 Id1
-        apply(auto simp add: ValueOfIdentifier_def)
-
-
-      then show ?thesis sorry
     next
       case L1 : (Literal v1)
 
